B4_group.v
@@ -3,7 +3,14 @@
 From CGT Require Import A1_setup B1_fmap B2_perm B3_word.
 Require Import Lia.
 
-Section Group.
+(***
+:: Groups ::
+
+The Schreier-Sims algorithm describes groups, but we want to avoid proving more
+Group Theory than strictly necessary. Therefore I favor short and efficient
+definitions over more mathematically complete ones.
+*)
+Section Groups.
 
 Notation can := (prune xH).
 Notation Canonical := (Pruned xH).
@@ -11,30 +18,31 @@ Notation Canonical := (Pruned xH).
 (* The generating set of the group. *)
 Variable gen : list perm.
 
-(* Range of the generator after n compositions. *)
-Fixpoint Generates n π :=
+(* Generator range for a bounded number of compositions. *)
+Fixpoint Generates_in n π :=
   match n with
   | O => can π = ident
-  | S m => ∃σ, In σ gen /\ Generates m (σ ∘ π)
+  | S m => ∃σ, In σ gen /\ Generates_in m (σ ∘ π)
   end.
 
-(* Group membership defined by the generator. *)
-Definition In_Group π := ∃n, Generates n π.
+(* Generator range for an unbounded number of compositions. *)
+Definition Generates π := ∃n, Generates_in n π.
 
-(* Cardinality of the group. *)
-Definition Group_Order (ord : positive) :=
-  ∃f : positive -> perm,
-    (∀i, i <= ord -> Canonical (f i)) /\
-    (∀π, In_Group π -> ∃i, i <= ord /\ f i = can π) /\
-    (∀i j, i <= ord -> j <= ord -> i ≠ j -> f i ≠ f j).
+(* The number of distinct permutations that are generated. *)
+Record Group_Order (ord : positive) := Group_Order_Witness {
+  enum : positive -> perm;
+  enum_canonical : ∀i, i <= ord -> Canonical (enum i);
+  enum_surjective : ∀π, Generates π -> ∃i, i <= ord /\ enum i = can π;
+  enum_injective : ∀i j, i <= ord -> j <= ord -> enum i = enum j -> i = j;
+}.
 
-End Group.
+End Groups.
 
 Theorem unit_group_order :
   Group_Order [] 1.
 Proof.
 exists (λ _, ident); repeat split; intros.
-2: lia. destruct H as [[]]; simpl in H.
+destruct H as [[]]; simpl in H.
 exists 1; split; easy.
-destruct H; easy.
+destruct H; easy. lia.
 Qed.
